src/Parsers/Refinement/DisjointRules.v
@@ -7,113 +7,16 @@ Require Import Fiat.Common.Equality.
 Require Import Fiat.Common.List.Operations.
 Require Import Fiat.Parsers.ContextFreeGrammar.ValidReflective.
 Require Import Fiat.Parsers.Refinement.DisjointLemmas.
+Require Import Fiat.Parsers.Refinement.DisjointRulesCommon.
 Require Import Fiat.Parsers.ParserInterface.
 Require Import Fiat.Parsers.StringLike.Core.
+Export DisjointLemmas.Exports.
 
 Set Implicit Arguments.
 
-Definition search_for_condition
-           {HSLM : StringLikeMin Ascii.ascii}
-           {HSL : StringLike Ascii.ascii}
-           {HSI : StringIso Ascii.ascii}
-           (G : pregrammar' Ascii.ascii)
-           str its (n : nat)
-  := is_first_char_such_that
-       (might_be_empty (possible_first_terminals_of_production G its))
-       str
-       n
-       (fun ch => list_bin ascii_beq ch (possible_first_terminals_of_production G its)).
-
-Lemma refine_disjoint_search_for'
-      {HSLM : StringLikeMin Ascii.ascii}
-      {HSL : StringLike Ascii.ascii}
-      {HSI : StringIso Ascii.ascii}
-      {HSLP : StringLikeProperties Ascii.ascii}
-      {HSIP : StringIsoProperties Ascii.ascii}
-      (G : pregrammar' Ascii.ascii)
-      (Hvalid : grammar_rvalid G)
-      {str offset len nt its}
-      (H_disjoint : disjoint ascii_beq
-                             (possible_terminals_of G nt)
-                             (possible_first_terminals_of_production G its))
-: refine {splits : list nat
-         | split_list_is_complete
-             G str offset len
-             (NonTerminal nt::its) splits}
-         (n <- { n : nat | n <= length (substring offset len str)
-                           /\ ((exists n', search_for_condition G (substring offset len str) its n')
-                               -> search_for_condition G (substring offset len str) its n) };
-          ret [n]).
-Proof.
-  intros ls H.
-  computes_to_inv; subst.
-  destruct H as [H0 H1].
-  apply PickComputes.
-  hnf; cbv zeta.
-  intros Hlen it' its' Heq n ? H_reachable pit pits.
-  inversion Heq; subst it' its'; clear Heq.
-  left.
-  pose proof (terminals_disjoint_search_for Hvalid _ H_disjoint pit pits H_reachable) as H'.
-  specialize (H1 (ex_intro _ n H')).
-  pose proof (is_first_char_such_that_eq_nat_iff H1 H') as H''.
-  destruct_head or; destruct_head and; subst;
-  rewrite ?Min.min_r, ?Min.min_l by assumption;
-  omega.
-Qed.
-
-Definition search_for_not_condition
-           {HSLM : StringLikeMin Ascii.ascii}
-           {HSL : StringLike Ascii.ascii}
-           {HSI : StringIso Ascii.ascii}
-           (G : pregrammar' Ascii.ascii)
-           str nt its n
-  := is_first_char_such_that
-       (might_be_empty (possible_first_terminals_of_production G its))
-       str
-       n
-       (fun ch => negb (list_bin ascii_beq ch (possible_terminals_of G nt))).
-
-Lemma refine_disjoint_search_for_not'
-      {HSLM : StringLikeMin Ascii.ascii}
-      {HSL : StringLike Ascii.ascii}
-      {HSI : StringIso Ascii.ascii}
-      {HSLP : StringLikeProperties Ascii.ascii}
-      {HSIP : StringIsoProperties Ascii.ascii}
-      {G : pregrammar' Ascii.ascii}
-      (Hvalid : grammar_rvalid G)
-      {str offset len nt its}
-      (H_disjoint : disjoint ascii_beq
-                             (possible_terminals_of G nt)
-                             (possible_first_terminals_of_production G its))
-: refine {splits : list nat
-         | split_list_is_complete
-             G str offset len
-             (NonTerminal nt::its)
-             splits}
-         (n <- { n : nat | n <= length (substring offset len str)
-                           /\ ((exists n', search_for_not_condition G (substring offset len str) nt its n')
-                               -> search_for_not_condition G (substring offset len str) nt its n) };
-          ret [n]).
-Proof.
-  intros ls H.
-  computes_to_inv; subst.
-  destruct H as [H0 H1].
-  apply PickComputes.
-  hnf; cbv zeta.
-  intros Hlen it' its' Heq n ? H_reachable pit pits.
-  inversion Heq; subst it' its'; clear Heq.
-  left.
-  pose proof (terminals_disjoint_search_for_not Hvalid _ H_disjoint pit pits H_reachable) as H'.
-  specialize (H1 (ex_intro _ n H')).
-  pose proof (is_first_char_such_that_eq_nat_iff H1 H') as H''.
-  destruct_head or; destruct_head and; subst;
-  rewrite ?Min.min_r by assumption;
-  omega.
-Qed.
-
 Lemma find_first_char_such_that'_short {Char HSLM HSL}
       str P len
-: @find_first_char_such_that' Char HSLM HSL P len str <= len.
+  : @find_first_char_such_that' Char HSLM HSL P len str <= len.
 Proof.
   revert str; induction len; simpl; intros; [ reflexivity | ].
   destruct (get (length str - S len) str) eqn:H.
@@ -124,7 +27,7 @@ Qed.
 
 Lemma find_first_char_such_that_short {Char HSLM HSL}
       str P
-: @find_first_char_such_that Char HSLM HSL str P <= length str.
+  : @find_first_char_such_that Char HSLM HSL str P <= length str.
 Proof.
   apply find_first_char_such_that'_short.
 Qed.
@@ -132,7 +35,7 @@ Qed.
 Lemma is_first_char_such_that__find_first_char_such_that {Char} {HSLM HSL} {HSLP : @StringLikeProperties Char HSLM HSL} str P
       might_be_empty
       (H : exists n, is_first_char_such_that might_be_empty str n (fun ch => is_true (P ch)))
-: is_first_char_such_that might_be_empty str (@find_first_char_such_that Char HSLM HSL str P) (fun ch => is_true (P ch)).
+  : is_first_char_such_that might_be_empty str (@find_first_char_such_that Char HSLM HSL str P) (fun ch => is_true (P ch)).
 Proof.
   unfold find_first_char_such_that.
   destruct H as [n H].
@@ -191,10 +94,10 @@ Lemma refine_find_first_char_such_that {Char} {HSLM : StringLikeMin Char} {HSL :
       (str : String)
       (P : Char -> bool)
       might_be_empty
-: refine { n : nat | n <= length str
-                     /\ ((exists n', is_first_char_such_that might_be_empty str n' P)
-                         -> is_first_char_such_that might_be_empty str n P) }
-         (ret (find_first_char_such_that str P)).
+  : refine { n : nat | n <= length str
+                       /\ ((exists n', is_first_char_such_that might_be_empty str n' P)
+                           -> is_first_char_such_that might_be_empty str n P) }
+           (ret (find_first_char_such_that str P)).
 Proof.
   intros v H.
   computes_to_inv; subst.
@@ -203,105 +106,173 @@ Proof.
   apply is_first_char_such_that__find_first_char_such_that.
 Qed.
 
-Lemma refine_disjoint_search_for
-      {HSLM : StringLikeMin Ascii.ascii}
-      {HSL : StringLike Ascii.ascii}
-      {HSI : StringIso Ascii.ascii}
-      {HSLP : StringLikeProperties Ascii.ascii}
-      {HSIP : StringIsoProperties Ascii.ascii}
-      {G : pregrammar' Ascii.ascii}
-      {str offset len nt its}
-      (Hvalid : grammar_rvalid G)
-      (H_disjoint : disjoint ascii_beq
-                             (possible_terminals_of G nt)
-                             (possible_first_terminals_of_production G its))
-: refine {splits : list nat
-         | split_list_is_complete
-             G str offset len
-             (NonTerminal nt::its)
-             splits}
-         (ret [find_first_char_such_that (substring offset len str) (fun ch => list_bin ascii_beq ch (possible_first_terminals_of_production G its))]).
-Proof.
-  rewrite refine_disjoint_search_for' by assumption.
-  setoid_rewrite refine_find_first_char_such_that.
-  simplify with monad laws; reflexivity.
-Qed.
+Section with_grammar.
+  Context {HSLM : StringLikeMin Ascii.ascii}
+          {HSL : StringLike Ascii.ascii}
+          {HSI : StringIso Ascii.ascii}
+          {HSLP : StringLikeProperties Ascii.ascii}
+          {HSIP : StringIsoProperties Ascii.ascii}
+          (G : pregrammar' Ascii.ascii)
+          (Hvalid : grammar_rvalid G)
+          (search_data : disjoint_search_data G).
 
-Lemma refine_disjoint_search_for_not
-      {HSLM : StringLikeMin Ascii.ascii}
-      {HSL : StringLike Ascii.ascii}
-      {HSI : StringIso Ascii.ascii}
-      {HSLP : StringLikeProperties Ascii.ascii}
-      {HSIP : StringIsoProperties Ascii.ascii}
-      {G : pregrammar' Ascii.ascii}
-      {str offset len nt its}
-      (Hvalid : grammar_rvalid G)
-      (H_disjoint : disjoint ascii_beq
-                             (possible_terminals_of G nt)
-                             (possible_first_terminals_of_production G its))
-: refine {splits : list nat
-         | split_list_is_complete
-             G str offset len
-             (NonTerminal nt::its)
-             splits}
-         (ret [find_first_char_such_that (substring offset len str) (fun ch => negb (list_bin ascii_beq ch (possible_terminals_of G nt)))]).
-Proof.
-  rewrite refine_disjoint_search_for_not' by assumption.
-  setoid_rewrite refine_find_first_char_such_that.
-  simplify with monad laws; reflexivity.
-Qed.
+  Local Notation possible_terminals_of := (possible_terminals_of G compiled_productions_possible_terminals).
+  Local Notation possible_first_terminals_of_production :=
+    (possible_first_terminals_of_production G compiled_productions_maybe_empty_of compiled_productions_possible_first_terminals).
+  Local Notation possible_terminals_of_production :=
+    (possible_terminals_of_production G compiled_productions_possible_terminals).
+  Local Notation possible_last_terminals_of :=
+    (possible_last_terminals_of G compiled_productions_maybe_empty_of compiled_productions_possible_last_terminals).
 
-Lemma refine_disjoint_search_for_idx
-      {HSLM : StringLikeMin Ascii.ascii}
-      {HSL : StringLike Ascii.ascii}
-      {HSI : StringIso Ascii.ascii}
-      {HSLP : StringLikeProperties Ascii.ascii}
-      {HSIP : StringIsoProperties Ascii.ascii}
-      {G : pregrammar' Ascii.ascii}
-      {str offset len nt its idx}
-      (Hvalid : grammar_rvalid G)
-      (Heq : default_to_production (G := G) idx = NonTerminal nt :: its)
-      (H_disjoint : disjoint ascii_beq
-                             (possible_terminals_of G nt)
-                             (possible_first_terminals_of_production G its))
-: refine {splits : list nat
-         | split_list_is_complete_idx
-             G str offset len
-             idx
-             splits}
-         (ret [find_first_char_such_that (substring offset len str) (fun ch => list_bin ascii_beq ch (possible_first_terminals_of_production G its))]).
-Proof.
-  unfold split_list_is_complete_idx.
-  erewrite <- refine_disjoint_search_for by eassumption.
-  rewrite Heq.
-  apply refine_pick_pick; intro; trivial.
-Qed.
+  Definition search_for_condition
+             str its (n : nat)
+    := is_first_char_such_that
+         (might_be_empty (possible_first_terminals_of_production its))
+         str
+         n
+         (fun ch => list_bin ascii_beq ch (possible_first_terminals_of_production its)).
 
-Lemma refine_disjoint_search_for_not_idx
-      {HSLM : StringLikeMin Ascii.ascii}
-      {HSL : StringLike Ascii.ascii}
-      {HSI : StringIso Ascii.ascii}
-      {HSLP : StringLikeProperties Ascii.ascii}
-      {HSIP : StringIsoProperties Ascii.ascii}
-      {G : pregrammar' Ascii.ascii}
-      {str offset len nt its idx}
-      (Hvalid : grammar_rvalid G)
-      (Heq : default_to_production (G := G) idx = NonTerminal nt :: its)
-      (H_disjoint : disjoint ascii_beq
-                             (possible_terminals_of G nt)
-                             (possible_first_terminals_of_production G its))
-: refine {splits : list nat
-         | split_list_is_complete_idx
-             G str offset len
-             idx
-             splits}
-         (ret [find_first_char_such_that (substring offset len str) (fun ch => negb (list_bin ascii_beq ch (possible_terminals_of G nt)))]).
-Proof.
-  unfold split_list_is_complete_idx.
-  erewrite <- refine_disjoint_search_for_not by eassumption.
-  rewrite Heq.
-  apply refine_pick_pick; intro; trivial.
-Qed.
+  Lemma refine_disjoint_search_for'
+        {str offset len nt its}
+        (H_disjoint : disjoint ascii_beq
+                               (possible_terminals_of nt)
+                               (possible_first_terminals_of_production its))
+    : refine {splits : list nat
+             | split_list_is_complete
+                 G str offset len
+                 (NonTerminal nt::its) splits}
+             (n <- { n : nat | n <= length (substring offset len str)
+                               /\ ((exists n', search_for_condition (substring offset len str) its n')
+                                   -> search_for_condition (substring offset len str) its n) };
+                ret [n]).
+  Proof.
+    intros ls H.
+    computes_to_inv; subst.
+    destruct H as [H0 H1].
+    apply PickComputes.
+    hnf; cbv zeta.
+    intros Hlen it' its' Heq n ? H_reachable pit pits.
+    inversion Heq; subst it' its'; clear Heq.
+    left.
+    pose proof (terminals_disjoint_search_for _ Hvalid _ H_disjoint pit pits H_reachable) as H'.
+    specialize (H1 (ex_intro _ n H')).
+    pose proof (is_first_char_such_that_eq_nat_iff H1 H') as H''.
+    destruct_head or; destruct_head and; subst;
+      rewrite ?Min.min_r, ?Min.min_l by assumption;
+      omega.
+  Qed.
+
+  Definition search_for_not_condition
+             str nt its n
+    := is_first_char_such_that
+         (might_be_empty (possible_first_terminals_of_production its))
+         str
+         n
+         (fun ch => negb (list_bin ascii_beq ch (possible_terminals_of nt))).
+
+  Lemma refine_disjoint_search_for_not'
+        {str offset len nt its}
+        (H_disjoint : disjoint ascii_beq
+                               (possible_terminals_of nt)
+                               (possible_first_terminals_of_production its))
+    : refine {splits : list nat
+             | split_list_is_complete
+                 G str offset len
+                 (NonTerminal nt::its)
+                 splits}
+             (n <- { n : nat | n <= length (substring offset len str)
+                               /\ ((exists n', search_for_not_condition (substring offset len str) nt its n')
+                                   -> search_for_not_condition (substring offset len str) nt its n) };
+                ret [n]).
+  Proof.
+    intros ls H.
+    computes_to_inv; subst.
+    destruct H as [H0 H1].
+    apply PickComputes.
+    hnf; cbv zeta.
+    intros Hlen it' its' Heq n ? H_reachable pit pits.
+    inversion Heq; subst it' its'; clear Heq.
+    left.
+    pose proof (terminals_disjoint_search_for_not _ Hvalid _ H_disjoint pit pits H_reachable) as H'.
+    specialize (H1 (ex_intro _ n H')).
+    pose proof (is_first_char_such_that_eq_nat_iff H1 H') as H''.
+    destruct_head or; destruct_head and; subst;
+      rewrite ?Min.min_r by assumption;
+      omega.
+  Qed.
+
+  Lemma refine_disjoint_search_for
+        {str offset len nt its}
+        (H_disjoint : disjoint ascii_beq
+                               (possible_terminals_of nt)
+                               (possible_first_terminals_of_production its))
+    : refine {splits : list nat
+             | split_list_is_complete
+                 G str offset len
+                 (NonTerminal nt::its)
+                 splits}
+             (ret [find_first_char_such_that (substring offset len str) (fun ch => list_bin ascii_beq ch (possible_first_terminals_of_production its))]).
+  Proof.
+    rewrite refine_disjoint_search_for' by assumption.
+    setoid_rewrite refine_find_first_char_such_that.
+    simplify with monad laws; reflexivity.
+  Qed.
+
+  Lemma refine_disjoint_search_for_not
+        {str offset len nt its}
+        (H_disjoint : disjoint ascii_beq
+                               (possible_terminals_of nt)
+                               (possible_first_terminals_of_production its))
+    : refine {splits : list nat
+             | split_list_is_complete
+                 G str offset len
+                 (NonTerminal nt::its)
+                 splits}
+             (ret [find_first_char_such_that (substring offset len str) (fun ch => negb (list_bin ascii_beq ch (possible_terminals_of nt)))]).
+  Proof.
+    rewrite refine_disjoint_search_for_not' by assumption.
+    setoid_rewrite refine_find_first_char_such_that.
+    simplify with monad laws; reflexivity.
+  Qed.
+
+  Lemma refine_disjoint_search_for_idx
+        {str offset len nt its idx}
+        (Heq : default_to_production (G := G) idx = NonTerminal nt :: its)
+        (H_disjoint : disjoint ascii_beq
+                               (possible_terminals_of nt)
+                               (possible_first_terminals_of_production its))
+    : refine {splits : list nat
+             | split_list_is_complete_idx
+                 G str offset len
+                 idx
+                 splits}
+             (ret [find_first_char_such_that (substring offset len str) (fun ch => list_bin ascii_beq ch (possible_first_terminals_of_production its))]).
+  Proof.
+    unfold split_list_is_complete_idx.
+    erewrite <- refine_disjoint_search_for by eassumption.
+    rewrite Heq.
+    apply refine_pick_pick; intro; trivial.
+  Qed.
+
+  Lemma refine_disjoint_search_for_not_idx
+        {str offset len nt its idx}
+        (Heq : default_to_production (G := G) idx = NonTerminal nt :: its)
+        (H_disjoint : disjoint ascii_beq
+                               (possible_terminals_of nt)
+                               (possible_first_terminals_of_production its))
+    : refine {splits : list nat
+             | split_list_is_complete_idx
+                 G str offset len
+                 idx
+                 splits}
+             (ret [find_first_char_such_that (substring offset len str) (fun ch => negb (list_bin ascii_beq ch (possible_terminals_of nt)))]).
+  Proof.
+    unfold split_list_is_complete_idx.
+    erewrite <- refine_disjoint_search_for_not by eassumption.
+    rewrite Heq.
+    apply refine_pick_pick; intro; trivial.
+  Qed.
+End with_grammar.
 
 Ltac solve_disjoint_side_conditions :=
   idtac;
@@ -321,26 +292,25 @@ Ltac replace_with_native_compute_in c H :=
 
 Ltac pose_disjoint_search_for lem :=
   idtac;
-  let G := match goal with |- appcontext[ParserInterface.split_list_is_complete_idx ?G ?str ?offset ?len ?idx] => G end in
-  let HSLM := match goal with |- appcontext[@ParserInterface.split_list_is_complete_idx ?Char ?G ?HSLM ?HSL] => HSLM end in
-  let HSL := match goal with |- appcontext[@ParserInterface.split_list_is_complete_idx ?Char ?G ?HSLM ?HSL] => HSL end in
-  let lem' := constr:(@refine_disjoint_search_for_idx HSLM HSL _ _ _ G) in
-  let H' := fresh in
-  assert (H' : ValidReflective.grammar_rvalid G) by (vm_compute; reflexivity);
+  let G := match goal with |- context[ParserInterface.split_list_is_complete_idx ?G ?str ?offset ?len ?idx] => G end in
+  let HSLM := match goal with |- context[@ParserInterface.split_list_is_complete_idx ?Char ?G ?HSLM ?HSL] => HSLM end in
+  let HSL := match goal with |- context[@ParserInterface.split_list_is_complete_idx ?Char ?G ?HSLM ?HSL] => HSL end in
+  let H' := get_hyp_of_shape (is_true (grammar_rvalid G)) in
+  let search_data := get_hyp_of_shape (disjoint_search_data G) in
+  let lem' := constr:(@refine_disjoint_search_for_idx HSLM HSL _ G H' search_data) in
   let lem' := match goal with
-              | [ |- appcontext[ParserInterface.split_list_is_complete_idx ?G ?str ?offset ?len ?idx] ]
-                => constr:(fun idx' nt its => lem' str offset len nt its idx' H')
+              | [ |- context[ParserInterface.split_list_is_complete_idx ?G ?str ?offset ?len ?idx] ]
+                => constr:(fun idx' nt its => lem' str offset len nt its idx')
               end in
-  pose proof lem' as lem;
-  clear H'.
+  pose proof lem' as lem.
 Ltac rewrite_once_disjoint_search_for_specialize lem lem' :=
   idtac;
   let G := (lazymatch goal with
-             | [ |- appcontext[ParserInterface.split_list_is_complete_idx ?G ?str ?offset ?len ?idx] ]
+             | [ |- context[ParserInterface.split_list_is_complete_idx ?G ?str ?offset ?len ?idx] ]
                => G
              end) in
   match goal with
-  | [ |- appcontext[ParserInterface.split_list_is_complete_idx ?G ?str ?offset ?len ?idx] ]
+  | [ |- context[ParserInterface.split_list_is_complete_idx G ?str ?offset ?len ?idx] ]
     => pose proof (lem idx) as lem';
        do 2 (lazymatch type of lem' with
               | forall a : ?T, _ => idtac; let x := fresh in evar (x : T); specialize (lem' x); subst x
@@ -374,3 +344,10 @@ Ltac rewrite_disjoint_search_for :=
   let lem := fresh "lem" in
   rewrite_disjoint_search_for_no_clear lem;
   clear lem.
+Ltac refine_disjoint_search_for :=
+  idtac;
+  let lem := fresh "lem" in
+  pose_disjoint_search_for lem;
+  let lem' := fresh "lem'" in
+  rewrite_once_disjoint_search_for_specialize lem lem';
+  refine lem'; clear lem'.
