src/Parsers/Refinement/DisjointLemmasEarlyDeclarations.v
@@ -1,0 +1,4 @@
+(** We declare this tactic here so we can overwrite it in
+    DisjointLemmas, but also run it in Refinement/Tactics.v without
+    importing DisjointLemmas. *)
+Ltac do_disjoint_precomputations _ := idtac.
